Completed formalization of Insertion Sort

RunTime/src/Formalization.lean
@@ -7,74 +7,142 @@ namespace counting
 
 @[simp] def ordered_insert (a : α) : list α → (list α × ℕ)
 | []       := ([a], 0)
-| (h :: t) := if a ≼ h then (a :: h :: t, 1)
-                       else let (l', n) := ordered_insert t in (h :: l', n + 1)
+| (h :: t) := if a ≼ h then (a :: h :: t, 0)
+                       else let (l', n) := ordered_insert t in (h :: l', 1 + n)
+
+#eval ordered_insert (λ m n : ℕ , m ≤ n) 2 [5, 3, 1, 4]
+-- ([2, 5, 3, 1, 4], 0)
+
+#eval ordered_insert (λ m n : ℕ , m ≤ n) 9 [1, 0, 8]
+-- ([1, 0, 8, 9], 3)
 
 @[simp] def insertion_sort : list α → (list α × ℕ)
 | [] := ([], 0)
 | (h :: t) := let (l', n) := (insertion_sort t) , (l'', m) := ordered_insert r h l'
               in (l'', n + m)
 
+#eval insertion_sort (λ m n : ℕ , m ≤ n) [1, 2, 3, 4, 5]
+-- ([1, 2, 3, 4, 5], 0)
+
+#eval insertion_sort (λ m n : ℕ , m ≤ n) [5, 4, 3, 2, 1]
+-- ([1, 2, 3, 4, 5], 10)
+
 @[simp] def smaller_prefix (a : α) : list α → ℕ
-| []       := 0
+| [] := 0
 | (h :: t) := if a ≼ h then 0 else 1 + smaller_prefix t
 
-end counting
+#eval smaller_prefix (λ m n : ℕ , m ≤ n) 6 [3, 1, 9, 4]
+-- 2
 
-theorem ordered_insert_linear (a : α) : ∀ l : list α, (counting.ordered_insert r a l).snd ≤ l.length :=
+#eval smaller_prefix (λ m n : ℕ , m ≤ n) 5 [6, 3, 2, 0]
+-- 0
+
+theorem ordered_insert_linear (a : α) :
+  ∀ l : list α, (ordered_insert r a l).snd ≤ l.length :=
 begin
   intro l,
   induction l,
   { simp, },
   { simp, split_ifs,
     { simp, },
-    { cases (counting.ordered_insert r a l_tl),
-      unfold counting.ordered_insert,
+    { cases (ordered_insert r a l_tl),
+      unfold ordered_insert,
+      linarith,
+    }
+  }
+end
+
+theorem ordered_insert_identification (a : α) : ∀ l : list α,
+  (ordered_insert r a l).fst = list.ordered_insert r a l :=
+begin
+  intro l,
+  induction l,
+  { simp, },
+  { simp, split_ifs,
+    { simp, },
+    { cases (ordered_insert r a l_tl),
+      unfold ordered_insert,
       simp,
       exact l_ih,
     }
   }
 end
 
-theorem ordered_insert_identification (a : α) : ∀ l : list α,
-  (counting.ordered_insert r a l).fst = list.ordered_insert r a l := sorry
-
-theorem counting_comparisons_ordered_insertion (a : α) : ∀ l : list α,
-  (counting.ordered_insert r a l).snd = counting.smaller_prefix (≼) a l
-| []       := by simp
-| (h :: t) :=
+theorem ordered_insert_length (a : α) : ∀ l : list α,
+  (ordered_insert r a l).fst.length = l.length + 1 :=
 begin
-  simp,
-  split_ifs,
-  { simp },
-  { rw counting_comparisons_oi t,
-    exact add_comm (counting.smaller_prefix r a t) 1
+  intro l,
+  rw ordered_insert_identification r a l,
+  exact list.ordered_insert_length r l a,
+end
+
+theorem comparisons_ordered_insertion (a : α) : ∀ l : list α,
+  (ordered_insert r a l).snd = smaller_prefix (≼) a l :=
+begin
+  intro l,
+  induction l,
+  { simp, },
+  { simp, split_ifs,
+    { exact rfl, },
+    { rw ← l_ih,
+      cases (ordered_insert r a l_tl),
+      unfold ordered_insert,
+    }
   }
 end
 
-#print counting.insertion_sort._match_1
-
-theorem insertion_sort_quadratic : ∀ l : list α, (counting.insertion_sort r l).snd ≤ (l.length * l.length) :=
+theorem insertion_sort_preserves_length : ∀ l : list α,
+  (insertion_sort r l).fst.length = l.length :=
 begin
   intro l,
   induction l,
   { simp, },
   { simp,
-    cases (counting.insertion_sort r l_tl) with sorted_tl ops,
-    unfold counting.insertion_sort,
-    have hh : (counting.ordered_insert r l_hd sorted_tl).snd ≤
+    cases (insertion_sort r l_tl) with sorted_tl _,
+    unfold insertion_sort,
+    have ordered_length :
+      (ordered_insert r l_hd sorted_tl).fst.length = sorted_tl.length + 1 :=
+      ordered_insert_length r l_hd sorted_tl,
+    cases (ordered_insert r l_hd sorted_tl) with sorted_list _,
+    unfold insertion_sort,
+    rw ordered_length,
+    rw l_ih,
+  }
+end
+
+theorem insertion_sort_quadratic : ∀ l : list α, (insertion_sort r l).snd ≤ l.length * l.length :=
+begin
+  intro l,
+  induction l,
+  { simp, },
+  { simp,
+    have same_lengths : (insertion_sort r l_tl).fst.length = l_tl.length :=
+      insertion_sort_preserves_length r l_tl,
+    cases (insertion_sort r l_tl) with sorted_tl ops,
+    unfold insertion_sort,
+    have hh : (ordered_insert r l_hd sorted_tl).snd ≤
        sorted_tl.length := ordered_insert_linear r l_hd sorted_tl,
-    cases (counting.ordered_insert r l_hd sorted_tl),
-    unfold counting.insertion_sort,
-    have same_lengths : sorted_tl.length = l_tl.length :=
-    begin
-      induction sorted_tl,
-      { sorry },
-      { sorry }
-    end,
+    cases (ordered_insert r l_hd sorted_tl),
+    unfold insertion_sort,
+
     linarith,
   }
 end
 
 theorem insertion_sort_identification (a : α) : ∀ l : list α,
-  (counting.insertion_sort r l).fst = list.insertion_sort r l := sorry
+  (insertion_sort r l).fst = list.insertion_sort r l :=
+begin
+  intro l,
+  induction l,
+  { simp, },
+  { simp,
+    rw ← l_ih,
+    cases insertion_sort r l_tl,
+    unfold insertion_sort,
+    rw ← ordered_insert_identification r l_hd fst,
+    cases ordered_insert r l_hd fst,
+    unfold insertion_sort,
+  }
+end
+
+end counting
